examples/iso_dh/impl.v
@@ -26,7 +26,7 @@ Definition iso_dhN := nroot.@"iso_dh".
 Definition mk_keyshare : val := λ: "k",
   texp (tint #0) "k".
 
-Definition initiator : val := λ: "c" "skI" "pkR" "N" "data",
+Definition initiator : val := λ: "c" "skI" "pkR" "N",
   let: "pkI"  := pkey "skI" in
   let: "a"    := mk_nonce #() in
   let: "ga"   := mk_keyshare "a" in
@@ -34,11 +34,11 @@ Definition initiator : val := λ: "c" "skI" "pkR" "N" "data",
   send "c" "m1";;
   bind: "m2"   := verify "pkR" (Tag $ iso_dhN.@"m2") (recv "c") in
   bind: "m2"   := list_of_term "m2" in
-  list_match: ["ga'"; "gb"; "pkI'"] := "m2" in
-  guard: eq_term "ga" "ga'" && eq_term "pkI" "pkI'" in
+  list_match: ["ga'"; "gb"; "pkI'"; "N'"] := "m2" in
+  guard: eq_term "ga" "ga'" && eq_term "pkI" "pkI'" && eq_term "N" "N'" in
   let: "gab" := texp "gb" "a" in
   let: "secret" := term_of_list ["pkI"; "pkR"; "ga"; "gb"; "gab"] in
-  let: "m3_body" := term_of_list ["ga"; "gb"; "pkR"; "N"; "data"] in
+  let: "m3_body" := term_of_list ["ga"; "gb"; "pkR"] in
   let: "m3" := sign "skI" (Tag $ iso_dhN.@"m3") "m3_body" in
   send "c" "m3";;
   SOME (derive_senc_key "secret").
@@ -56,22 +56,19 @@ Definition responder_accept : val := λ: "c" "skR" "ga" "pkI" "N",
   let: "b" := mk_nonce #() in
   let: "gb" := mk_keyshare "b" in
   let: "m2" := sign "skR" (Tag $ iso_dhN.@"m2")
-                 (term_of_list ["ga"; "gb"; "pkI"]) in
+                 (term_of_list ["ga"; "gb"; "pkI"; "N"]) in
   send "c" "m2";;
   bind: "m3" := verify "pkI" (Tag $ iso_dhN.@"m3") (recv "c") in
   bind: "m3" := list_of_term "m3" in
-  list_match: ["ga'"; "gb'"; "pkR'"; "N'"; "data"] := "m3" in
-  guard: eq_term "ga" "ga'" && eq_term "gb" "gb'" && eq_term "pkR" "pkR'"
-         && eq_term "N" "N'" in
+  list_match: ["ga'"; "gb'"; "pkR'"] := "m3" in
+  guard: eq_term "ga" "ga'" && eq_term "gb" "gb'" && eq_term "pkR" "pkR'" in
   let: "gab" := texp "ga" "b" in
   let: "secret" := term_of_list ["pkI"; "pkR"; "ga"; "gb"; "gab"] in
-  SOME (derive_senc_key "secret", "data").
+  SOME (derive_senc_key "secret").
 
 Definition responder : val := λ: "c" "skR" "N",
   let: "res" := responder_wait "c" in
   let: "ga"  := Fst "res" in
   let: "pkI" := Snd "res" in
-  bind: "res" := responder_accept "c" "skR" "ga" "pkI" "N" in
-  let: "kS" := Fst "res" in
-  let: "data" := Snd "res" in
-  SOME ("pkI", "kS", "data").
+  bind: "kS" := responder_accept "c" "skR" "ga" "pkI" "N" in
+  SOME ("pkI", "kS").
