examples/iso_dh/proofs/responder.v
@@ -24,7 +24,6 @@ Implicit Types (failed : bool).
 Implicit Types (si : sess_info) (osi : option sess_info).
 Implicit Types (N : namespace) (data : term).
 Implicit Types (ores : option (term * term)).
-Implicit Types (oresa : option (term * term * term)).
 
 Ltac protocol_failure :=
   by intros; wp_pures; iApply ("Hpost" $! None); iFrame.
@@ -52,26 +51,25 @@ Lemma wp_responder_accept failed c skI skR ga N φ :
   {{{ channel c ∗ cryptis_ctx ∗
       iso_dh_ctx ∗ iso_dh_pred N φ ∗
       public ga ∗ minted skI ∗ minted skR ∗
+      (∀ gb, term_token gb (↑iso_dhN.@"res") ={⊤}=∗ φ gb) ∗
       if failed then public skI ∨ public skR
       else True }}}
     responder_accept c skR ga (Spec.pkey skI) (Tag N)
-  {{{ ores, RET (repr ores);
-      if ores is Some (kS, data) then ∃ si,
+  {{{ okS, RET (repr okS);
+      if okS is Some kS then ∃ si,
         ⌜si_init si = skI⌝ ∗
         ⌜si_resp si = skR⌝ ∗
         ⌜kS = si_key si⌝ ∗
         minted (si_key si) ∗
-        public data ∗
         session Resp si ∗
         □ (⌜failed⌝ → compromised_session Resp si) ∗
         release_token (si_resp_share si) ∗
-        term_token (si_resp_share si) (⊤ ∖ ↑iso_dhN) ∗
-        ((public skI ∨ public skR) ∨ φ data)
+        term_token (si_resp_share si) (⊤ ∖ ↑iso_dhN)
       else True }}}.
 Proof.
 set pkR := Spec.pkey skR.
 iIntros "%Φ (#chan_c & #? & (#? & #?) & #N_φ &
-             #p_ga & #m_skI & #m_skR & #failed) Hpost".
+             #p_ga & #m_skI & #m_skR & res & #failed) Hpost".
 wp_lam. wp_pures. wp_apply wp_pkey. wp_pures.
 wp_apply (wp_mk_nonce_freshN ∅
           (λ b, ⌜failed⌝ ∨ released ga ∧ released (TExp (TInt 0) b))%I
@@ -90,8 +88,10 @@ rewrite big_sepS_singleton.
 iDestruct (release_tokenI with "token") as "[token_rel token]" => //.
 rewrite (term_token_difference gb (↑iso_dhN.@"failed")); last by solve_ndisj.
 iDestruct "token" as "[token_failed token]".
-iPoseProof (term_token_difference gb (↑iso_dhN.@"ready") with "token")
-  as "[token_ready token]"; first by solve_ndisj.
+iPoseProof (term_token_difference gb (↑iso_dhN.@"res") with "token")
+  as "[res_token token]"; first by solve_ndisj.
+iMod ("res" with "res_token") as "res".
+iMod (iso_dh_ready_alloc ga with "[//] res") as "#ready".
 iAssert (public gb) as "#p_gb".
 { iApply public_TExp_iff; eauto.
   rewrite minted_TInt. iRight. do ![iSplit => //].
@@ -102,9 +102,10 @@ wp_apply wp_mk_keyshare => //.
 iIntros "_". wp_pures. wp_list. wp_term_of_list.
 wp_apply wp_sign; eauto.
 { rewrite public_of_list /=. do !iSplit => //.
-  by rewrite public_verify_key. }
+  - by rewrite public_verify_key.
+  - by rewrite public_Tag. }
 { iRight. iModIntro.
-  iExists ga, b, _. do ![iSplitR => //].
+  iExists ga, b, _, N. do ![iSplitR => //].
   case: failed; eauto.
   rewrite bi.False_or. by eauto. }
 iIntros "%m2 #?". wp_pures. wp_apply wp_send; eauto.
@@ -113,13 +114,11 @@ wp_apply wp_verify; eauto. iSplit; last by protocol_failure.
 iIntros "{p_m3} %m3' #p_m3 #inv_m3".
 set pkI := Spec.pkey skI.
 wp_pures. wp_list_of_term m3'; last by protocol_failure.
-wp_list_match => [ga' gb' pkR' N' data -> {m3}|]; last by protocol_failure.
+wp_list_match => [ga' gb' pkR' -> {m3}|]; last by protocol_failure.
 wp_eq_term e; last by protocol_failure. subst ga'.
 wp_eq_term e; last by protocol_failure. subst gb'.
 wp_eq_term e; last by protocol_failure. subst pkR'.
-wp_eq_term e; last by protocol_failure. subst N'.
 rewrite public_of_list /=.
-iDestruct "p_m3" as "(_ & _ & _ & _ & p_data & _)".
 wp_pure _ credit:"H3".
 wp_apply wp_texp.
 wp_pure _ credit:"H4".
@@ -135,34 +134,29 @@ iAssert (▷ (⌜failed⌝ ∨ released_session si) → public (si_key si))%I as
   - iApply public_TExp => //. by iApply "s_b". }
 iAssert (|={⊤}=>
            □ (⌜failed⌝ → compromised_session Resp si) ∗
-           ((public (si_init si) ∨ public (si_resp si)) ∨ φ data) ∗
            ∃ failed,
              term_meta gb (iso_dhN.@"failed") failed ∗
              if failed then
                public (si_init si) ∨ public (si_resp si)
              else □ (public (si_key si) → ▷ released_session si))%I
-  with "[token_failed token_ready H4]" as "> (#comp & res & i_m3)".
+  with "[token_failed H4]" as "> (#comp & i_m3)".
 { case: failed.
   { iMod (term_meta_set (iso_dhN.@"failed") true with "token_failed")
       as "#?"; first by solve_ndisj.
     iAssert (compromised_session Resp si) as "#?".
     { do !iSplit => //. iApply "s_k1". by eauto. }
-    iModIntro. iSplit; first by eauto. iSplit; first by eauto.
+    iModIntro. iSplit; first by eauto.
     iExists true. by eauto. }
   iDestruct "inv_m3" as "[comp|#inv]".
   { iMod (term_meta_set (iso_dhN.@"failed") true with "token_failed")
       as "#?"; first by solve_ndisj.
     iModIntro. iSplit; first by iIntros "!> []".
-    iSplit; eauto.
     iExists true. iSplit => //. by eauto. }
-  iDestruct "inv"
-    as "(%a & %gb' & %skR' & %N' & %data' & %e_m3 & comp & ready)".
+  iDestruct "inv" as "(%a & %gb' & %skR' & %e_m3 & comp)".
   case/Spec.of_list_inj: e_m3
-    => -> <- /Spec.sign_pkey_inj <- /Tag_inj <- <- {ga gb' skR' N' data'}
+    => -> <- /Spec.sign_pkey_inj <- {ga gb' skR'}
     in gb gab si *.
   rewrite !TExp_TExpN TExpC2 in gab si *.
-  iMod ("ready" with "[//] token_ready") as "{ready} ready".
-  iMod (lc_fupd_elim_later with "H4 ready") as "ready".
   iDestruct "comp" as "[comp|comp]".
   - iMod (term_meta_set (iso_dhN.@"failed") true with "token_failed")
       as "#?"; first by solve_ndisj.
@@ -178,7 +172,7 @@ iAssert (minted (si_key si)) as "#m_kS".
   - by iApply public_verify_key.
   - by iApply public_verify_key. }
 wp_pures.
-iApply ("Hpost" $! (Some (si_key si : term, data))).
+iApply ("Hpost" $! (Some (si_key si))).
 iModIntro. iFrame. iExists si. iFrame. do !iSplit => //.
 - iIntros "!> #?". iApply "s_k1". by eauto.
 - iApply (term_token_drop with "token"). solve_ndisj.
@@ -190,14 +184,13 @@ Lemma wp_responder_accept_weak c skR ga skI N :
       minted skR ∗ minted skI ∗
       public ga }}}
     responder_accept c skR ga (Spec.pkey skI) (Tag N)
-  {{{ ores,
-      RET (repr ores);
-      if ores is Some (kS, data) then ∃ si,
+  {{{ okS,
+      RET (repr okS);
+      if okS is Some kS then ∃ si,
         ⌜si_init si = skI⌝ ∗
         ⌜si_resp si = skR⌝ ∗
         ⌜kS = si_key si⌝ ∗
         minted (si_key si) ∗
-        public data ∗
         ((public (si_init si) ∨ public (si_resp si))
            ∨ □ (public (si_key si) ↔ ▷ False)) ∗
         term_token (si_resp_share si) (⊤ ∖ ↑iso_dhN)
@@ -207,10 +200,10 @@ Proof.
 iIntros "%Φ (#chan_c & #ctx & #? & #? & #m_skR & #m_skI & #p_ga) Hpost".
 iApply wp_fupd. wp_apply (wp_responder_accept false); first by eauto 10.
 iIntros "%osi Hsi".
-case: osi => [[kS data]|]; last by iApply ("Hpost" $! None).
-iDestruct "Hsi" as "(%si & <- & <- & -> & #m_kS & #? & #sec & #? & rel & tok & _)".
+case: osi => [kS|]; last by iApply ("Hpost" $! None).
+iDestruct "Hsi" as "(%si & <- & <- & -> & #m_kS & #sec & #? & rel & tok)".
 iMod (unrelease with "rel") as "#un". iModIntro.
-iApply ("Hpost" $! (Some (si_key si : term, data))). iFrame. do !iSplit => //.
+iApply ("Hpost" $! (Some (si_key si))). iFrame. do !iSplit => //.
 iDestruct "sec" as "(? & %failed & ? & ?)".
 case: failed; eauto.
 iRight. iApply (unreleased_key_secrecy Resp) => //.
@@ -222,7 +215,7 @@ Lemma wp_responder c skR N :
       iso_dh_ctx ∗ iso_dh_pred N (λ _, True)%I ∗ minted skR }}}
     responder c skR (Tag N)
   {{{ oresa, RET (repr oresa);
-      if oresa is Some (pkI, kS, data) then ∃ si,
+      if oresa is Some (pkI, kS) then ∃ si,
         ⌜pkI = Spec.pkey (si_init si)⌝ ∗
         ⌜si_resp si = skR⌝ ∗
         ⌜kS = si_key si⌝ ∗
@@ -241,9 +234,9 @@ iIntros "%ga %skI (#p_ga & #m_skI)".
 wp_pures.
 wp_apply (wp_responder_accept false); first by eauto 10.
 iIntros "%osi Hosi".
-case: osi => [[kS data]|]; wp_pures; last by iApply ("post" $! None).
-iDestruct "Hosi" as "(%si & <- & <- & -> & #? & #? & #? & #? & rel & token & _)".
-iModIntro. iApply ("post" $! (Some (Spec.pkey _, si_key si : term, data))).
+case: osi => [kS|]; wp_pures; last by iApply ("post" $! None).
+iDestruct "Hosi" as "(%si & <- & <- & -> & #? & #? & #? & rel & token)".
+iModIntro. iApply ("post" $! (Some (Spec.pkey _, si_key si))).
 iExists si. iFrame. by eauto 10.
 Qed.
 
